\title{Formulas}
\author{Barry Wittman}


\documentclass[12pt]{article}


\usepackage{amsmath}

%\usepackage{kmath}
%\usepackage[math]{anttor}
%\usepackage{millennial}
%\usepackage{fouriernc}
%\usepackage[varg]{txfonts}
\usepackage[charter]{mathdesign}
%\usepackage{fourier}

\usepackage{noto}
\usepackage[T1]{fontenc}

\begin{document}

$$
M = P \cdot \frac{J}{1 - (1 + J)^{-N}}
$$

$$
\frac{-b \pm \sqrt{b^2 - 4ac}}{2a}
$$


\begin{align*}
x &= \frac{n}{x} \\
x^2 &= n \\
x &= \sqrt{n}
\end{align*}

$$
\begin{bmatrix}
1 & 0 & 0 \\
0 & \cos \theta & -\sin \theta \\
0 & \sin \theta  & \cos \theta \\
\end{bmatrix}
$$

$$
v'_i = \sum_{j = 1}^n A_{ij}\cdot v_j
$$

$$
\sigma = \sqrt{\frac{1}{n - 1}\sum_{i = 1}^n (x_i - \mu)^2}
$$

$$
f(x) = \sqrt{x}
$$

$$
F = \frac{Gm_1m_2}{r^2}
$$

$$
d = \sqrt{(x_1 - x_2)^2 + (y_1 - y_2)^2 + (z_1 -  z_2)^2}
$$

$$
d = \sqrt{(x_1 - x_2)^2+(y_1 - y_2)^2}
$$

$$
\mathbf{F}_{ab} = - G \frac{m_a m_b}{{\vert \mathbf{r}_{ab} \vert}^2} \, \mathbf{\hat{r}}_{ab}
$$

$$
\mathbf{\hat{r}}_{ab} = \frac{\mathbf{r}_b - \mathbf{r}_a}{\vert\mathbf{r}_b - \mathbf{r}_a\vert}
$$

$$
S = \sum_{i=1}^N f\left(a_i\right)
$$

$$
S_1 = \sum_{i=1}^{\lfloor \frac{N}{2}\rfloor } f\left(a_i\right)\hspace{.75in}
S_2 = \sum_{i=\lfloor \frac{N}{2} \rfloor +1}^{N} f\left(a_i\right)
$$

$$
\mbox{speedup}=\frac{t_s}{t_c} = \frac{4,100}{1,660,000} = 0.00246
$$

$$
C_{ij} = \sum_{k = 1}^n A_{ik}B_{kj} = A_{i1}B_{1j} + A_{i2}B_{2j} + \ldots + A_{in}B_{nj}
$$

$$
y = \sqrt{r^2 - x^2}
$$

$$
F = k_\mathrm{e} \frac{q_1q_2}{r^2}
$$

$$
E = k_\mathrm{e} \frac{q}{r^2}
$$

$$
age(year) =
\left\{\begin{array}{lll}
0 & \text{if you were born in $year$} &  \text{(Base Case)} \\
1 + age(year-1) & \text{if you were born before $year$} &  \text{(Recursive Case)}
\end{array}\right.
$$

$$
x \cdot y =
\left\{\begin{array}{lll}
x & \text{if  $y = 1$} & \text{(Base Case)} \\
x + \left(x \cdot (y - 1)\right) & \text{if $y > 1$} & \text{(Recursive Case)}
\end{array}\right.
$$

$$
n! =
\left\{\begin{array}{lll}
1 & \text{if  $n = 0$} & \text{(Base Case)} \\
n \cdot (n-1)! & \text{if $n>0$} & \text{(Recursive Case)}
\end{array}\right.
$$

$$
F_n =
\left\{\begin{array}{lll}
1 & \text{if  $n=0$ or  $n = 1$} & \text{(Base Cases)} \\
F_{n-1}+F_{n-2} & \text{if $n>1$} & \text{(Recursive Case)}
\end{array}\right.
$$

$$
a^n =
\left\{\begin{array}{lll}
a & \text{if $n=1$} & \text{(Base case)} \\
a \cdot a^{n - 1} & \text{if $n>1$} & \text{(Recursive case)}
\end{array}\right.
$$

$$
a^n =
\left\{\begin{array}{lll}
a & \text{if  $n=1$} & \text{(Base Case)} \\
\left(a^{\frac{n}{2}}\right)^2 & \text{if  $n>1$} & \text{(Recursive Case)}
\end{array}\right.
$$

$$
\begin{aligned}
\left(\frac{1}{2}\right)^x \cdot n &= 1\\
2^x\left(\frac{1}{2}\right)^x \cdot n &= 2^x\\
n &= 2^x\\
2^k &= 2^x\\
k &= x\\
\log_2 n &= x\\
\end{aligned}
$$

$$
a^n =
\left\{\begin{array}{lll}
a & \text{if  $n=1$} & \text{(Base Case)} \\
\left(a^{\frac{n}{2}}\right)^2 & \text{if  $n>1$ and even} & \text{(Recursive Case)} \\
a\cdot \left(a^{\frac{n - 1}{2}}\right)^2 & \text{if  $n>1$ and odd} & \text{(Recursive Case)}
\end{array}\right.
$$

$$
F_n = \frac{\left(\frac{1 + \sqrt{5}}{2}\right)^{n+1}  -  \left(\frac{1 -
\sqrt{5}}{2}\right)^{n+1}}{\sqrt{5}}
$$


\end{document}