\title{Formulas}
\author{Barry Wittman}


\documentclass[12pt]{article}


\usepackage{amsmath}

%\usepackage{kmath}
%\usepackage[math]{anttor}
%\usepackage{millennial}
%\usepackage{fouriernc}
%\usepackage[varg]{txfonts}
\usepackage[charter]{mathdesign}
%\usepackage{fourier}

\usepackage{noto}
\usepackage[T1]{fontenc}

\begin{document}

$$
\begin{aligned}
\left(\frac{1}{2}\right)^x \cdot n &= 1\\
2^x\left(\frac{1}{2}\right)^x \cdot n &= 2^x\\
n &= 2^x\\
2^k &= 2^x\\
k &= x\\
\log_2 n &= x\\
\end{aligned}
$$

$$
a^n =
\left\{\begin{array}{lll}
a & \text{if  $n=1$} & \text{(Base Case)} \\
\left(a^{\frac{n}{2}}\right)^2 & \text{if  $n>1$ and even} & \text{(Recursive Case)} \\
a\cdot \left(a^{\frac{n - 1}{2}}\right)^2 & \text{if  $n>1$ and odd} & \text{(Recursive Case)}
\end{array}\right.
$$

$$
F_n = \frac{\left(\frac{1 + \sqrt{5}}{2}\right)^{n+1}  -  \left(\frac{1 -
\sqrt{5}}{2}\right)^{n+1}}{\sqrt{5}}
$$


\end{document}